Add an executable normalization function for terms

theories/par.v
@@ -1,4 +1,5 @@
 Require Export imports.
+From stdpp Require Import relations (rtc(..) , sn).
 
 Inductive TyPar : Ty -> Ty -> Type :=
 | TP_Var i :
@@ -58,6 +59,58 @@ with SNRed : Tm -> Tm -> Prop :=
   SN b ->
   SNRed (TmApp (TmAbs a) b) (subst_Tm (b…) a).
 
+Definition isAbs a :=
+  match a with
+  | TmAbs _ => true
+  | _ => false
+  end.
+
+Fixpoint nf a :=
+  match a with
+  | VarTm _ => true
+  | TmApp b a => ne b && nf a
+  | TmAbs b => nf b
+  end
+with ne a :=
+  match a with
+  | VarTm _ => true
+  | TmApp b a => ne b && nf a
+  | TmAbs _ => false
+  end.
+
+Inductive Red : Tm -> Tm -> Prop :=
+| R_AppAbs b a  :
+  Red (TmApp (TmAbs b) a) (subst_Tm (a…) b)
+| R_App0 b0 b1 a :
+  ~~ isAbs b0 ->
+  Red b0 b1 ->
+  Red (TmApp b0 a) (TmApp b1 a)
+| R_App1 b a0 a1 :
+  ne b ->
+  Red a0 a1 ->
+  Red (TmApp b a0) (TmApp b a1)
+| R_Abs b0 b1 :
+  Red b0 b1 ->
+  Red (TmAbs b0) (TmAbs b1).
+
+Inductive FRed : Tm -> Tm -> Prop :=
+| F_AppAbs b a  :
+  FRed (TmApp (TmAbs b) a) (subst_Tm (a…) b)
+| F_App0 b0 b1 a :
+  FRed b0 b1 ->
+  FRed (TmApp b0 a) (TmApp b1 a)
+| F_App1 b a0 a1 :
+  FRed a0 a1 ->
+  FRed (TmApp b a0) (TmApp b a1)
+| F_Abs b0 b1 :
+  FRed b0 b1 ->
+  FRed (TmAbs b0) (TmAbs b1).
+
+Lemma ne_nf : forall a, ne a -> nf a.
+Proof.
+  elim => //=.
+Qed.
+
 Scheme SN_ind_2 := Minimality for SN Sort Prop
                    with SNe_ind_2 := Minimality for SNe Sort Prop
                     with redSN_ind_2 := Minimality for SNRed Sort Prop.
@@ -114,6 +167,129 @@ Module red_props.
       have -> : subst_Tm (VarTm i…) a0 = ren_Tm (i…) a0 by substify; asimpl.
       qauto use:antirenaming.
   Qed.
+
+  Lemma Rs_Abs a0 a1 :
+    rtc Red a0 a1 ->
+    rtc Red (TmAbs a0) (TmAbs a1).
+  Proof.
+    induction 1; qauto ctrs:rtc use:R_Abs.
+  Qed.
+
+  Lemma Red_IsAbs a0 a1 :
+    rtc Red a0 a1 ->
+    isAbs a0 -> isAbs a1.
+    induction 1 => //=.
+    - hauto lq:on inv:Red ctrs:rtc.
+  Qed.
+
+  Lemma Rs_App b0 b1 a0 a1 :
+    rtc Red b0 b1 ->
+    rtc Red a0 a1 ->
+    ne b1 ->
+    rtc Red (TmApp b0 a0) (TmApp b1 a1).
+    move => h. move : a0 a1. elim : b0 b1 /h.
+    - move => + a0 a1 h.
+      elim : a0 a1 /h; hauto lq:on ctrs:rtc, Red.
+    - move => b0 b1 b2 hb hb' ih a0 a1 ha hb2.
+      apply rtc_l with (y := (TmApp b1 a0)); eauto.
+      apply R_App0; eauto. apply /negP => h.
+      have : isAbs b2 by hauto lq:on use:Red_IsAbs ctrs:rtc.
+      move : hb2; clear. case : b2 => //=.
+  Qed.
+
+  Lemma sn_red :
+    (forall a, SN a -> exists b, nf b /\ rtc Red a b) /\
+    (forall a, SNe a -> exists b, ne b /\ rtc Red a b) /\
+      (forall a b, SNRed a b -> Red a b).
+    apply SN_multind.
+    - sfirstorder use:ne_nf.
+    - sfirstorder use:Rs_Abs.
+    - hauto q:on ctrs:rtc.
+    - move => i.
+      exists (VarTm i).
+      eauto using rtc_refl.
+    - move => a b ha [a0 ha0] hb [b0 hb0].
+      exists (TmApp a0 b0).
+      split => /=.
+      sfirstorder b:on.
+      sfirstorder use:Rs_App.
+    - hauto lq:on rew:off inv:SNRed ctrs:Red.
+    - qauto use:R_AppAbs.
+  Qed.
+
+  Fixpoint redf a : option Tm :=
+    match a with
+    | VarTm _ => None
+    | TmAbs a => match redf a with
+                | Some a => Some (TmAbs a)
+                | None => None
+                end
+    | TmApp (TmAbs b) a => Some (subst_Tm (a…) b)
+    | TmApp b a => match redf b with
+                  | Some b => Some (TmApp b a)
+                  | None => match redf a with
+                           | Some a => Some (TmApp b a)
+                           | None => None
+                           end
+                  end
+    end.
+
+  Lemma nf_ne_red a :
+    ne a \/ nf a -> redf a = None.
+    elim : a => //=; hauto lqb:on.
+  Qed.
+
+  Lemma Red_red a b : Red a b -> redf a = Some b.
+  Proof.
+    move => h. elim : a b /h.
+    - done.
+    - hauto lq:on rew:off.
+    - hauto lq:on rew:off use:nf_ne_red.
+    - hauto lq:on.
+  Qed.
+
+  Polymorphic Inductive IsAbs {A : Type} (a : Tm) (b1 : A) (F : Tm -> A) : A -> Tm -> Prop :=
+  | IsAbsTrue a0 :  IsAbs a b1 F (F a0) (TmAbs a0)
+  | isAbsFalse  : ~~ isAbs a -> IsAbs a b1 F b1 a.
+
+  Polymorphic Lemma IsAbsP {A : Type} a (b1 : A) F :
+    let e := match a with
+             | TmAbs a => F a
+             | _ => b1
+             end in
+    IsAbs a b1 F e a.
+  Proof. hauto lq:on ctrs:IsAbs inv:Tm. Qed.
+
+  Lemma red_FRed a b : redf a = Some b -> FRed a b.
+  Proof.
+    elim : a b => //=.
+    - hauto q:on ctrs:FRed.
+    - hauto lq:on rew:off inv:Tm ctrs:FRed.
+  Qed.
+
+  Lemma SN_red_sn a : SN a -> sn (fun a b => redf a = Some b) a.
+  Proof.
+    move => h. apply sn_red in h.
+    move : h => [v [hv hr]].
+    move : hv.
+    elim : a v / hr.
+    - hauto q:on ctrs:Acc use:nf_ne_red.
+    - move => a b c h0 h1 ih hc.
+      apply Acc_intro => /= a'.
+      move /Red_red in h0.
+      move => ?. have ? : a' = b by congruence. subst.
+      by apply ih.
+  Qed.
+
+  Definition normalize a : SN a -> {x : Tm | rtc FRed a x}.
+    intros h.
+    apply SN_red_sn in h.
+    induction h as [x h ih].
+    destruct (redf x) as [x0 | ] eqn:eq.
+    destruct (ih x0 eq) as [x1 h1].
+    - exists x1. apply : rtc_l; eauto. apply red_FRed. apply eq.
+    - exists x. apply rtc_refl.
+  Defined.
 
   Lemma CR_Prod s0 s1 : CR s0 -> CR s1 -> CR (fun b => forall a, s0 a -> s1 (TmApp b a)).
   Proof.
